src/Init/Data/Iterators/Lemmas/Combinators.lean
@@ -6,5 +6,5 @@ Authors: Paul Reichert
 module
 
 prelude
-import Init.Data.Iterators.Lemmas.Consumers
-import Init.Data.Iterators.Lemmas.Combinators
+import Init.Data.Iterators.Lemmas.Combinators.Monadic
+import Init.Data.Iterators.Lemmas.Combinators.FilterMap
