src/Init/Data/Iterators/Lemmas/Combinators/Monadic.lean
@@ -6,5 +6,4 @@ Authors: Paul Reichert
 module
 
 prelude
-import Init.Data.Iterators.Lemmas.Consumers
-import Init.Data.Iterators.Lemmas.Combinators
+import Init.Data.Iterators.Lemmas.Combinators.Monadic.FilterMap
